Language

src/Language.v
@@ -3,56 +3,91 @@
 (* ON SEPERATION LOGIC *)
 (* Author: Hans-Dieter A. Hiep *)
 
-From Coq Require Import ZArith.
-From Coq Require Import FunctionalExtensionality.
-From Coq Require Import ProofIrrelevance.
-From Coq Require Import Ensembles.
-From Coq Require Import List.
+Require Import FunctionalExtensionality.
+Require Import PropExtensionality.
+Require Import Ensembles.
+Require Import List.
+Require Import ZArith.
 
-Definition SomeZ (v: Z) := Some v.
-Coercion SomeZ: Z >-> option.
+Require Import OnSeparationLogic.Heap.
 
-Definition L := Z.
+Module Language (Export HS: HeapSig).
 
-Record heap: Set := mkheap {
-  hfun: L -> option Z;
-  hvar: list L;
-  hcond: forall x, In x hvar <-> hfun x <> None
-}.
-Coercion hfun: heap >-> Funclass.
-
-Definition dom (h: heap): Ensemble L :=
-  fun n => h n <> None.
-
-Definition Partition (h h1 h2: heap): Prop :=
-  ((Included Z (dom h) (Union Z (dom h1) (dom h2)) /\
-    Disjoint Z (dom h1) (dom h2)) /\
-   (forall n, dom h1 n -> h n = h1 n)) /\
-  (forall n, dom h2 n -> h n = h2 n).
-
-Definition hfun_update (h: heap) (n: L) (v: Z): L -> option Z :=
-  fun m => if Z.eq_dec n m then v else h m.
-Definition hvar_update (h: heap) (n: L) (v: Z): list L :=
-  cons n (hvar h).
-Proposition hcond_update (h: heap) (n: L) (v: Z):
-    forall x, In x (hvar_update h n v) <-> (hfun_update h n v) x <> None.
-split; unfold hvar_update; unfold hfun_update; intro.
-- destruct H.
-  rewrite H; destruct (Z.eq_dec x x).
-  intro; inversion H0.
-  exfalso; apply n0; reflexivity.
-  unfold hfun_update.
-  destruct (Z.eq_dec n x).
-  intro; inversion H0.
-  apply hcond; assumption.
-- destruct (Z.eq_dec n x).
-  rewrite e; constructor; reflexivity.
-  right. apply hcond; assumption.
-Qed.
-Definition heap_update (h: heap) (n: L) (v: Z): heap :=
-  mkheap (hfun_update h n v) (hvar_update h n v) (hcond_update h n v).
+Module H := HeapFacts HS.
+Export H.
 
 Definition V := nat.
+Definition dummy: V := 0.
+
+Fixpoint maximum (xs: list V): V :=
+  match xs with
+  | nil => dummy
+  | (x::xs) => max x (maximum xs)
+  end.
+Proposition maximum_prop (xs: list V):
+  forall x, In x xs -> x <= maximum xs.
+intros. induction xs. inversion H.
+simpl. destruct H.
+rewrite H.
+apply Nat.le_max_l.
+destruct (le_gt_dec a (maximum xs)).
+rewrite max_r; try assumption.
+apply IHxs; assumption.
+unfold gt in g.
+apply Nat.lt_le_incl in g.
+rewrite max_l; try assumption.
+eapply le_trans.
+apply IHxs; assumption.
+assumption.
+Qed.
+
+Proposition maximum_app (xs ys: list V):
+  maximum (xs ++ ys) = max (maximum xs) (maximum ys).
+induction xs; simpl. reflexivity.
+rewrite IHxs.
+apply Nat.max_assoc.
+Qed.
+
+Definition fresh (xs: list V): V := S (maximum xs).
+Proposition fresh_prop (xs: list V):
+  forall x, In x xs -> x < fresh xs.
+unfold fresh.
+intros. apply le_lt_n_Sm.
+apply maximum_prop; assumption.
+Qed.
+Proposition fresh_notIn (xs: list V):
+  ~In (fresh xs) xs.
+intro.
+pose proof (fresh_prop xs).
+specialize H0 with (fresh xs).
+specialize (H0 H).
+eapply Nat.lt_irrefl. apply H0.
+Qed.
+
+Proposition fresh_app (xs ys: list V):
+  fresh (xs ++ ys) = max (fresh xs) (fresh ys).
+unfold fresh.
+rewrite maximum_app.
+simpl. reflexivity.
+Qed.
+
+Proposition fresh_notInApp (xs ys: list V):
+  ~In (fresh (xs ++ ys)) xs.
+rewrite fresh_app.
+destruct (Nat.max_dec (fresh xs) (fresh ys)).
+rewrite e. apply fresh_notIn.
+rewrite e.
+pose proof (Max.le_max_l (fresh xs) (fresh ys)).
+rewrite e in H.
+destruct (Nat.eq_dec (fresh xs) (fresh ys)).
+rewrite <- e0. apply fresh_notIn.
+apply Nat.le_lteq in H. destruct H. clear n.
+intro.
+apply fresh_prop in H0.
+eapply Nat.lt_irrefl.
+eapply Nat.lt_trans. apply H. apply H0.
+exfalso. apply n. assumption.
+Qed.
 
 Definition store := V -> Z.
 
@@ -62,13 +97,44 @@ Definition store_update (s: store) (x: V) (v: Z): store :=
 Definition eq_restr (s t: store) (z: list V): Prop :=
   forall (x: V), In x z -> s x = t x.
 
-(* Expressions are shallow, but finitely based *)
+Proposition eq_restr_split (s t: store) (xs ys: list V):
+  eq_restr s t (xs ++ ys) -> eq_restr s t xs /\ eq_restr s t ys.
+unfold eq_restr; intro; split; intros;
+apply H; apply in_or_app; auto.
+Qed.
+
+(* Expressions and guards are shallow, but finitely based *)
 Record expr: Set := mkexpr {
   eval: store -> Z;
   evar: list V;
   econd: forall (s t: store), eq_restr s t evar -> eval s = eval t
 }.
 Coercion eval: expr >-> Funclass.
+
+Proposition const_expr_cond (v: Z) (s t : store):
+  eq_restr s t nil -> v = v.
+intros. reflexivity.
+Qed.
+Definition const_expr (v: Z): expr :=
+  mkexpr (fun s => v) nil (const_expr_cond v).
+Coercion const_expr: Z >-> expr.
+Proposition var_expr_cond (x: V) (s t : store):
+  eq_restr s t (x :: nil) -> s x = t x.
+intro. unfold eq_restr in H.
+specialize H with x. apply H.
+left. reflexivity.
+Qed.
+Definition var_expr (x: V): expr :=
+  mkexpr (fun s => s x) (x :: nil) (var_expr_cond x).
+Coercion var_expr: V >-> expr.
+
+Proposition expr_eq (e1 e2: expr):
+  (eval e1 = eval e2) -> (evar e1 = evar e2) -> e1 = e2.
+intros. destruct e1. destruct e2.
+simpl in *. revert econd0. rewrite H. rewrite H0.
+intro. pose proof (proof_irrelevance _ econd0 econd1).
+rewrite H1. reflexivity.
+Qed.
 
 Record guard: Set := mkguard {
   gval: store -> bool;
@@ -84,6 +150,27 @@ Qed.
 Definition const_guard (v: bool): guard :=
   mkguard (fun s => v) nil (const_guard_cond v).
 Coercion const_guard: bool >-> guard.
+Proposition equals_cond (e1 e2: expr) (s t : store):
+  eq_restr s t (evar e1 ++ evar e2) ->
+  (if Z.eq_dec (eval e1 s) (eval e2 s) then true else false) =
+  (if Z.eq_dec (eval e1 t) (eval e2 t) then true else false).
+intro H.
+apply eq_restr_split in H; destruct H.
+pose proof (econd e1 s t); rewrite H1.
+pose proof (econd e2 s t); rewrite H2.
+all: auto.
+Qed.
+Definition equals (e1 e2: expr): guard :=
+  mkguard (fun s => if Z.eq_dec (eval e1 s) (eval e2 s) then
+    true else false) (evar e1 ++ evar e2) (equals_cond e1 e2).
+
+Proposition guard_eq (g1 g2: guard):
+  (gval g1 = gval g2) -> (gvar g1 = gvar g2) -> g1 = g2.
+intros. destruct g1. destruct g2.
+simpl in *. revert gcond0. rewrite H. rewrite H0.
+intro. pose proof (proof_irrelevance _ gcond0 gcond1).
+rewrite H1. reflexivity.
+Qed.
 
 Inductive assert :=
 | test: guard -> assert
@@ -98,48 +185,19 @@ Coercion test: guard >-> assert.
 Definition lnot (p: assert): assert := (limp p false).
 Definition lor (p q: assert): assert := lnot (land (lnot p) (lnot q)).
 Definition lexists (x: V) (p: assert): assert := lnot (lforall x (lnot p)).
+Definition hasvaldash (e: expr): assert :=
+  let y := fresh (evar e) in lexists y (hasval e y).
+Definition emp: assert := (lforall dummy (lnot (hasvaldash dummy))).
+Definition pointsto (e e': expr): assert :=
+  let x := fresh (evar e) in land (hasval e e') (lforall x (limp (hasvaldash x) (equals x e))).
+Definition pointstodash (e: expr): assert :=
+  let y := fresh (evar e) in lexists y (pointsto e y).
+Definition hasval_alt (e e': expr): assert :=
+  sand (pointsto e e') true.
+Definition hasvaldash_alt (e: expr): assert :=
+  sand (pointstodash e) true.
 
-(* Classical *)
-
-Fixpoint satisfy (h: heap) (s: store) (p: assert): Prop :=
-  match p with
-  | test g => g s = true
-  | hasval e e' => dom h (e s) /\ h (e s) = e' s
-  | land p q => satisfy h s p /\ satisfy h s q
-  | limp p q => satisfy h s p -> satisfy h s q
-  | lforall x p => forall v, satisfy h (store_update s x v) p
-  | sand p q => exists h1 h2, Partition h h1 h2 /\
-      satisfy h1 s p /\ satisfy h2 s q
-  | simp p q => forall h'' h', Partition h'' h h' ->
-      satisfy h' s p -> satisfy h'' s q
-  end.
-
-(* Stable assertions *)
-Definition stable (p: assert) := forall h s, satisfy h s (lnot (lnot p)) -> satisfy h s p.
-
-Proposition stable_simp (p q: assert): stable p -> stable q -> stable (simp p q).
-intros.
-unfold stable; intros.
-simpl; intros.
-apply H0.
-simpl; intros.
-simpl in H1; apply H1; intro.
-apply H4.
-eapply H5. apply H2. assumption.
-Qed.
-
-Fixpoint satisfy_i (h: heap) (s: store) (p: assert): Prop :=
-  match p with
-  | test g => g s = true
-  | hasval e e' => dom h (e s) /\ h (e s) = e' s
-  | land p q => satisfy_i h s p /\ satisfy_i h s q
-  | limp p q => forall h'' h', Partition h'' h h' -> satisfy_i h' s p -> satisfy_i h' s q
-  | lforall x p => forall v, satisfy_i h (store_update s x v) p
-  | sand p q => exists h1 h2, Partition h h1 h2 /\
-      satisfy_i h1 s p /\ satisfy_i h2 s q
-  | simp p q => forall h'' h', Partition h'' h h' ->
-      satisfy_i h' s p -> satisfy_i h'' s q
-  end.
+End Language.
 
 
 
